Fix the IL1 proofs
They had broken due to changes in the semantics necessary to get the IL2
proofs through.

compiler/proofs/toIntLang1ProofScript.sml
@@ -1632,15 +1632,15 @@ val letrec_global_env = Q.prove (
      >- metis_tac [letrec_global_env_lem3]));
 
 val dec_to_i1_correct = Q.prove (
-`!mn mods tops d menv cenv env s s' r genv s_i1 next' tops' d_i1.
+`!mn mods tops d menv cenv env s s' r genv s_i1 next' tops' d_i1 tdecs tdecs'.
   r ≠ Rerr Rtype_error ∧
-  evaluate_dec mn (menv,cenv,env) s d (s',r) ∧
+  evaluate_dec mn (menv,cenv,env) (s,tdecs) d ((s',tdecs'),r) ∧
   global_env_inv genv mods tops menv {} env ∧
   s_to_i1' genv s s_i1 ∧
   dec_to_i1 (LENGTH genv) mn mods tops d = (next',tops',d_i1)
   ⇒
   ?s'_i1 r_i1.
-    evaluate_dec_i1 genv cenv s_i1 d_i1 (s'_i1,r_i1) ∧
+    evaluate_dec_i1 genv cenv (s_i1,tdecs) d_i1 ((s'_i1,tdecs'),r_i1) ∧
     (!cenv' env'.
       r = Rval (cenv',env')
       ⇒
@@ -1719,7 +1719,7 @@ val dec_to_i1_correct = Q.prove (
      cases_on `pmatch_i1 cenv s''' p v'' []` >>
      fs [match_result_to_i1_def] >>
      rw [] >>
-     MAP_EVERY qexists_tac [`s'''`, `Rerr (Rraise (Conv_i1 (SOME ("Bind",TypeExn NONE)) []))`] >>
+     MAP_EVERY qexists_tac [`s'''`, `Rerr (Rraise (Conv_i1 (SOME ("Bind",TypeExn (Short "Bind"))) []))`] >>
      rw []
      >- (ONCE_REWRITE_TAC [evaluate_i1_cases] >>
          rw [] >>
@@ -1834,16 +1834,16 @@ val decs_to_i1_num_bindings = Q.prove (
  decide_tac);
 
 val decs_to_i1_correct = Q.prove (
-`!mn mods tops ds menv cenv env s s' r genv s_i1 s'_i1 next' tops' ds_i1 cenv'.
+`!mn mods tops ds menv cenv env s s' r genv s_i1 tdecs s'_i1 tdecs' next' tops' ds_i1 cenv'.
   r ≠ Rerr Rtype_error ∧
-  evaluate_decs mn (menv,cenv,env) s ds (s',cenv',r) ∧
+  evaluate_decs mn (menv,cenv,env) (s,tdecs) ds ((s',tdecs'),cenv',r) ∧
   global_env_inv genv mods tops menv {} env ∧
   s_to_i1' genv s s_i1 ∧
   decs_to_i1 (LENGTH genv) mn mods tops ds = (next',tops',ds_i1)
   ⇒
   ∃s'_i1 new_genv new_genv' new_env' r_i1.
    new_genv' = MAP SND new_genv ∧
-   evaluate_decs_i1 genv cenv s_i1 ds_i1 (s'_i1,cenv',new_genv',r_i1) ∧
+   evaluate_decs_i1 genv cenv (s_i1,tdecs) ds_i1 ((s'_i1,tdecs'),cenv',new_genv',r_i1) ∧
    s_to_i1' (genv ++ new_genv') s' s'_i1 ∧
    (!new_env.
      r = Rval new_env
@@ -1869,6 +1869,8 @@ val decs_to_i1_correct = Q.prove (
  `?next' tops' d_i1. dec_to_i1 (LENGTH genv) mn mods tops h = (next',tops',d_i1)` by metis_tac [pair_CASES] >>
  fs [] >>
  rw [] >>
+ `?s2' tdecs2. s2 = (s2',tdecs2)` by metis_tac [pair_CASES] >>
+ fs [] >>
  imp_res_tac dec_to_i1_correct >>
  pop_assum mp_tac >>
  rw [] >>
@@ -1904,13 +1906,13 @@ val decs_to_i1_correct = Q.prove (
              by metis_tac [v_to_i1_weakening, global_env_inv_extend2] >>
      FIRST_X_ASSUM (qspecl_then [`mn`, `mods`, `tops |++ tops''`, `menv`, 
                                  `merge_envC ([],new_tds) cenv`, `new_env ++ env`,
-                                 `s2`, `s'`, `r'`, `genv ++ MAP SND env'_i1`, `s'_i1`,
-                                 `next'`, `tops'''`, `ds_i1'`, `new_tds'`] mp_tac) >>
+                                 `s2'`, `s'`, `r'`, `genv ++ MAP SND env'_i1`, `s'_i1`,
+                                 `tdecs2`, `tdecs'`, `next'`, `tops'''`, `ds_i1'`, `new_tds'`] mp_tac) >>
      rw [merge_def] >>
      MAP_EVERY qexists_tac [`s'_i1'`, `env'_i1++new_genv`, `r_i1`] >>
      rw []
      >- (disj2_tac >>
-         MAP_EVERY qexists_tac [`s'_i1`, `new_tds'`, `new_tds`, `MAP SND env'_i1`, `MAP SND new_genv`] >>
+         MAP_EVERY qexists_tac [`(s'_i1,tdecs2)`, `new_tds'`, `new_tds`, `MAP SND env'_i1`, `MAP SND new_genv`] >>
          rw [combine_dec_result_def, merge_def, MAP_REVERSE])
      >- (cases_on `r'` >>
          fs [combine_dec_result_def])
@@ -1958,17 +1960,18 @@ val global_env_inv_extend_mod = Q.prove (
 
 val global_env_inv_extend_mod_err = Q.prove (
 `!genv new_genv mods tops tops' menv new_env env mn new_genv'.
+  mn ∉ set (MAP FST menv) ∧
   global_env_inv genv mods tops menv ∅ env
   ⇒
   global_env_inv (genv ++ MAP SND new_genv ++ new_genv')
-                 (mods |+ (mn,FEMPTY |++ tops')) tops ((mn,[])::menv) ∅ env`,
+                 (mods |+ (mn,FEMPTY |++ tops')) tops menv ∅ env`,
  rw [last (CONJUNCTS v_to_i1_eqns)]
  >- metis_tac [v_to_i1_weakening] >>
- every_case_tac >>
- rw [FLOOKUP_UPDATE] >>
+ rw [FLOOKUP_UPDATE]
+ >- metis_tac [lookup_in2] >>
  fs [v_to_i1_eqns] >>
+ rw [] >>
  res_tac >>
- qexists_tac `map` >>
  rw [] >>
  res_tac  >>
  qexists_tac `n` >>
@@ -1976,36 +1979,35 @@ val global_env_inv_extend_mod_err = Q.prove (
  >- decide_tac >>
  metis_tac [v_to_i1_weakening, EL_APPEND1, APPEND_ASSOC]);
 
-val add_empty_mod_def = Define `
-(add_empty_mod (Tdec _) menv = menv) ∧
-(add_empty_mod (Tmod mn _ _) menv = (mn,[])::menv)`;
-
-val top_to_i1_correct = Q.prove (
-`!mods tops t menv cenv env s s' r genv s_i1 next' tops' mods' prompt_i1 cenv'.
-  r ≠ Rerr Rtype_error ∧
-  evaluate_top (menv,cenv,env) s t (s',cenv',r) ∧
+val to_i1_invariant_def = Define `
+to_i1_invariant genv mods tops menv env s s_i1 mod_names ⇔
+  set (MAP FST menv) ⊆ mod_names ∧
   global_env_inv genv mods tops menv {} env ∧
-  s_to_i1' genv s s_i1 ∧
+  s_to_i1' genv s s_i1`;
+
+val top_to_i1_correct = Q.store_thm ("top_to_i1_correct",
+`!mods tops t menv cenv env s s' r genv s_i1 next' tops' mods' prompt_i1 cenv' tdecs tdecs' mod_names mod_names'.
+  r ≠ Rerr Rtype_error ∧
+  to_i1_invariant genv mods tops menv env s s_i1 mod_names ∧
+  evaluate_top (menv,cenv,env) (s,tdecs,mod_names) t ((s',tdecs',mod_names'),cenv',r) ∧
   top_to_i1 (LENGTH genv) mods tops t = (next',mods',tops',prompt_i1)
   ⇒
   ∃s'_i1 new_genv r_i1.
-   evaluate_prompt_i1 genv cenv s_i1 prompt_i1 (s'_i1,cenv',new_genv,r_i1) ∧
-   s_to_i1' (genv ++ new_genv) s' s'_i1 ∧
+   evaluate_prompt_i1 genv cenv (s_i1,tdecs,mod_names) prompt_i1 ((s'_i1,tdecs',mod_names'),cenv',new_genv,r_i1) ∧
    next' = LENGTH  (genv ++ new_genv) ∧
    (!new_menv new_env.
      r = Rval (new_menv, new_env)
      ⇒
      r_i1 = NONE ∧
-     next' = LENGTH (genv++new_genv) ∧
-     global_env_inv (genv ++ new_genv) mods' tops' (new_menv ++ menv) {} (new_env ++ env)) ∧
+     to_i1_invariant (genv ++ new_genv) mods' tops' (new_menv++menv) (new_env++env) s' s'_i1 mod_names') ∧
    (!err.
      r = Rerr err
      ⇒
      ?err_i1.
        r_i1 = SOME err_i1 ∧
        result_to_i1 (\a b c. T) (genv ++ new_genv) (Rerr err) (Rerr err_i1) ∧
-       global_env_inv (genv ++ new_genv) mods' tops (add_empty_mod t menv) {} (env))`,
- rw [evaluate_top_cases, evaluate_prompt_i1_cases, top_to_i1_def, LET_THM] >>
+       to_i1_invariant (genv ++ new_genv) mods' tops menv env s' s'_i1 mod_names')`,
+ rw [evaluate_top_cases, evaluate_prompt_i1_cases, top_to_i1_def, LET_THM, to_i1_invariant_def] >>
  fs [] >>
  rw []
  >- (`?next'' tops'' d_i1. dec_to_i1 (LENGTH genv) NONE mods tops d = (next'',tops'',d_i1)` by metis_tac [pair_CASES] >>
@@ -2013,12 +2015,10 @@ val top_to_i1_correct = Q.prove (
      rw [] >>
      imp_res_tac dec_to_i1_correct >>
      fs [result_to_i1_cases] >>
-     `?new_tds' env'. v' = (new_tds',env')` by metis_tac [pair_CASES] >>
-     rw [] >>
      fs [fupdate_list_foldl] >>
      rw [] >>
      MAP_EVERY qexists_tac [`s'_i1`, `MAP SND env'_i1`] >>
-     rw [emp_def, mod_cenv_def] >>
+     rw [emp_def, mod_cenv_def, update_mod_state_def] >>
      rw [Once evaluate_decs_i1_cases] >>
      rw [Once evaluate_decs_i1_cases, emp_def, merge_def] >>
      fs [] >>
@@ -2034,21 +2034,20 @@ val top_to_i1_correct = Q.prove (
      rw [] >>
      fs [fupdate_list_foldl] >>
      fs [] >>
-     rw [decs_to_cenv_i1_def]
+     rw []
      >- (MAP_EVERY qexists_tac [`s'_i1`, `GENLIST (\n. Litv_i1 Unit) (decs_to_dummy_env [d_i1])`, `SOME (Rraise v')`] >>
          rw []
          >- (ONCE_REWRITE_TAC [evaluate_decs_i1_cases] >>
              rw [] >>
              ONCE_REWRITE_TAC [evaluate_decs_i1_cases] >>
              rw [] >>
-             fs [evaluate_dec_i1_cases] >>
-             rw [emp_def, dec_to_cenv_i1_def])
-         >- metis_tac [s_to_i1'_cases, v_to_i1_weakening]
+             fs [] >>
+             rw [emp_def, update_mod_state_def])
          >- (rw [decs_to_dummy_env_def] >>
              metis_tac [dec_to_i1_num_bindings])
          >- metis_tac [s_to_i1'_cases, v_to_i1_weakening]
-         >- (rw [add_empty_mod_def, decs_to_dummy_env_def] >>
-             metis_tac [v_to_i1_weakening]))
+         >- metis_tac [s_to_i1'_cases, v_to_i1_weakening]
+         >- metis_tac [s_to_i1'_cases, v_to_i1_weakening])
      >- (MAP_EVERY qexists_tac [`s'_i1`, `GENLIST (\n. Litv_i1 Unit) (decs_to_dummy_env [d_i1])`] >>
          rw []
          >- (ONCE_REWRITE_TAC [evaluate_decs_i1_cases] >>
@@ -2056,12 +2055,11 @@ val top_to_i1_correct = Q.prove (
              ONCE_REWRITE_TAC [evaluate_decs_i1_cases] >>
              rw [] >>
              fs [evaluate_dec_i1_cases] >>
-             rw [emp_def, dec_to_cenv_i1_def])
-         >- metis_tac [s_to_i1'_cases, v_to_i1_weakening]
+             rw [emp_def, update_mod_state_def])
          >- (rw [decs_to_dummy_env_def] >>
              metis_tac [dec_to_i1_num_bindings])
-         >- (rw [add_empty_mod_def, decs_to_dummy_env_def] >>
-             metis_tac [v_to_i1_weakening])))
+         >- metis_tac [s_to_i1'_cases, v_to_i1_weakening]
+         >- metis_tac [s_to_i1'_cases, v_to_i1_weakening]))
  >- (`?next'' tops'' ds_i1. decs_to_i1 (LENGTH genv) (SOME mn) mods tops ds = (next'',tops'',ds_i1)` by metis_tac [pair_CASES] >>
      fs [] >>
      rw [] >>
@@ -2069,7 +2067,8 @@ val top_to_i1_correct = Q.prove (
      fs [] >>
      rw [mod_cenv_def, emp_def] >>
      MAP_EVERY qexists_tac [`s'_i1`, `MAP SND new_genv`] >>
-     rw [fupdate_list_foldl] >>
+     rw [fupdate_list_foldl, update_mod_state_def] >>
+     fs [SUBSET_DEF] >>
      metis_tac [global_env_inv_extend_mod])
  >- (`?next'' tops'' ds_i1. decs_to_i1 (LENGTH genv) (SOME mn) mods tops ds = (next'',tops'',ds_i1)` by metis_tac [pair_CASES] >>
      fs [] >>
@@ -2082,33 +2081,35 @@ val top_to_i1_correct = Q.prove (
                             `SOME err_i1`] >>
      rw [] 
      >- (MAP_EVERY qexists_tac [`MAP SND new_genv`] >>
-         rw [])
-     >- metis_tac [s_to_i1'_cases, v_to_i1_weakening]
+         rw [update_mod_state_def])
      >- (imp_res_tac decs_to_i1_num_bindings >>
          decide_tac)
      >- (fs [result_to_i1_cases] >>
          rw [] >>
          metis_tac [s_to_i1'_cases, v_to_i1_weakening])
-     >- (rw [add_empty_mod_def, fupdate_list_foldl] >>
-         metis_tac [global_env_inv_extend_mod_err])));
+     >- fs [SUBSET_DEF]
+     >- (rw [fupdate_list_foldl] >>
+         `mn ∉ set (MAP FST menv)` 
+                    by (fs [SUBSET_DEF] >>
+                        metis_tac []) >>
+         metis_tac [global_env_inv_extend_mod_err])
+     >- metis_tac [s_to_i1'_cases, v_to_i1_weakening]));
 
-val prog_to_i1_correct = Q.prove (
-`!mods tops menv cenv env s prog s' r genv s_i1 next' tops' mods'  cenv' prog_i1.
+val prog_to_i1_correct = Q.store_thm ("prog_to_i1_correct",
+`!mods tops menv cenv env s prog s' r genv s_i1 next' tops' mods'  cenv' prog_i1 tdecs mod_names tdecs' mod_names'.
   r ≠ Rerr Rtype_error ∧
-  evaluate_prog (menv,cenv,env) s prog (s',cenv',r) ∧
-  global_env_inv genv mods tops menv {} env ∧
-  s_to_i1' genv s s_i1 ∧
+  evaluate_prog (menv,cenv,env) (s,tdecs,mod_names) prog ((s',tdecs',mod_names'),cenv',r) ∧
+  to_i1_invariant genv mods tops menv env s s_i1 mod_names ∧
   prog_to_i1 (LENGTH genv) mods tops prog = (next',mods',tops',prog_i1)
   ⇒
   ∃s'_i1 new_genv r_i1.
-   evaluate_prog_i1 genv cenv s_i1 prog_i1 (s'_i1,cenv',new_genv,r_i1) ∧
+   evaluate_prog_i1 genv cenv (s_i1,tdecs,mod_names) prog_i1 ((s'_i1,tdecs',mod_names'),cenv',new_genv,r_i1) ∧
    (!new_menv new_env.
      r = Rval (new_menv, new_env)
      ⇒
-     r_i1 = NONE ∧
-     s_to_i1' (genv ++ new_genv) s' s'_i1 ∧
      next' = LENGTH  (genv ++ new_genv) ∧
-     global_env_inv (genv ++ new_genv) mods' tops' (new_menv ++ menv) {} (new_env ++ env)) ∧
+     r_i1 = NONE ∧
+     to_i1_invariant (genv ++ new_genv) mods' tops' (new_menv++menv) (new_env++env) s' s'_i1 mod_names') ∧
    (!err.
      r = Rerr err
      ⇒
@@ -2125,21 +2126,25 @@ val prog_to_i1_correct = Q.prove (
  rw [] >>
  qpat_assum `evaluate_prog a b c d` (mp_tac o SIMP_RULE (srw_ss()) [Once evaluate_prog_cases]) >>
  rw [] >>
- rw [Once evaluate_prog_i1_cases]
- >- (`?s'_i1 new_genv.
-       evaluate_prompt_i1 genv cenv s_i1 prompt_i1 (s'_i1,new_tds,new_genv,NONE) ∧
-       s_to_i1' (genv ++ new_genv) s2 s'_i1 ∧
-       next'' = LENGTH (genv ++ new_genv) ∧
-       global_env_inv (genv ++ new_genv) mods'' tops'' (new_mods ++ menv) ∅ (new_env ++ env)`
-                 by metis_tac [top_to_i1_correct, result_distinct] >>
+ rw [Once evaluate_prog_i1_cases] >>
+ `?s2' tdecs2' mod_names2'. s2 = (s2',tdecs2',mod_names2')` by metis_tac [pair_CASES] >>
+ rw []
+ >- (`∃s'_i1 new_genv.
+      evaluate_prompt_i1 genv cenv (s_i1,tdecs,mod_names) prompt_i1
+         ((s'_i1,tdecs2',mod_names2'),new_tds,new_genv,NONE) ∧
+      next'' = LENGTH genv + LENGTH new_genv ∧
+      to_i1_invariant (genv ++ new_genv) mods'' tops'' (new_mods ++ menv) (new_env ++ env) s2' s'_i1 mod_names2'`
+                 by (imp_res_tac top_to_i1_correct >>
+                     fs [] >>
+                     metis_tac []) >>
      fs [merge_def] >>
-     FIRST_X_ASSUM (qspecl_then [`mods''`, `tops''`, `new_mods ++ menv`,`merge_envC new_tds cenv`,`new_env ++ env`, `s2`, `s'`,
-                                 `r'`, `genv++new_genv`, `s'_i1`] mp_tac) >>
+     FIRST_X_ASSUM (qspecl_then [`mods''`, `tops''`, `new_mods ++ menv`, `merge_envC new_tds cenv`, `new_env ++ env`, `s2'`, `s'`, `r'`, `genv++new_genv`, `s'_i1`] mp_tac) >>
+     rw [] >>
+     FIRST_X_ASSUM (qspecl_then [`new_tds'`, `tdecs2'`, `mod_names2'`, `tdecs'`, `mod_names'`] mp_tac) >>
      rw [] >>
      `r' ≠ Rerr Rtype_error` 
             by (Cases_on `r'` >>
                 fs [combine_mod_result_def]) >>
-     FIRST_X_ASSUM (qspecl_then [`new_tds'`] mp_tac) >>
      rw [] >>
      cases_on `r'` >>
      fs [combine_mod_result_def]
@@ -2151,13 +2156,13 @@ val prog_to_i1_correct = Q.prove (
          metis_tac [])
      >- (fs [result_to_i1_cases] >>
          rw [] >>
-         metis_tac [v_to_i1_weakening, APPEND_ASSOC]))
+         metis_tac [v_to_i1_weakening, APPEND_ASSOC, LENGTH_APPEND]))
  >- (imp_res_tac top_to_i1_correct >>
      pop_assum mp_tac >>
      rw [] >>
      fs [result_to_i1_cases] >>
      rw [] >>
-     metis_tac [v_to_i1_weakening, APPEND_ASSOC]));
+     metis_tac [v_to_i1_weakening, APPEND_ASSOC, LENGTH_APPEND]));
 
 val init_mods_def = Define `
   init_mods = FEMPTY`;
@@ -2188,5 +2193,10 @@ val initial_i1_invariant = Q.prove (
               metis_tac [])) >>
      fs [])
  >- rw [v_to_i1_eqns, s_to_i1'_cases]);
+
+val init_to_i1_invariant = Q.store_thm ("init_to_i1_invariant",
+`to_i1_invariant init_genv init_mods init_tops [] init_env [] [] {}`,
+ rw [to_i1_invariant_def] >>
+ metis_tac [initial_i1_invariant]);
 
 val _ = export_theory ();
