compiler/intLang1Script.sml
@@ -676,47 +676,55 @@ evaluate_match_i1 ck (genv,cenv,env) (count,s) v ((p,e)::pes) err_v ((count,s), 
 ==>
 evaluate_match_i1 ck env s v ((p,e)::pes) err_v (s, Rerr Rtype_error))`;
 
-val _ = Hol_reln ` (! genv cenv n e vs s1 s2 count.
+val _ = Hol_reln ` (! genv cenv n e vs s1 s2 count tdecs.
 (evaluate_i1 F (genv,cenv,emp) ( 0,s1) e ((count,s2), Rval (Conv_i1 NONE vs)) /\
 (LENGTH vs = n))
 ==>
-evaluate_dec_i1 genv cenv s1 (Dlet_i1 n e) (s2, Rval (emp, vs)))
+evaluate_dec_i1 genv cenv (s1,tdecs) (Dlet_i1 n e) ((s2,tdecs), Rval (emp, vs)))
 
-/\ (! genv cenv n e vs s1 s2 count.
+/\ (! genv cenv n e vs s1 s2 count tdecs.
 (evaluate_i1 F (genv,cenv,emp) ( 0,s1) e ((count,s2), Rval (Conv_i1 NONE vs)) /\ ~ ((LENGTH vs) = n))
 ==>
-evaluate_dec_i1 genv cenv s1 (Dlet_i1 n e) (s2, Rerr Rtype_error))
+evaluate_dec_i1 genv cenv (s1,tdecs) (Dlet_i1 n e) ((s2,tdecs), Rerr Rtype_error))
 
-/\ (! genv cenv n e v s1 s2 count.
+/\ (! genv cenv n e v s1 s2 count tdecs.
 (evaluate_i1 F (genv,cenv,emp) ( 0,s1) e ((count,s2), Rval v) /\
 ~ (? vs. v = Conv_i1 NONE vs))
 ==>
-evaluate_dec_i1 genv cenv s1 (Dlet_i1 n e) (s2, Rerr Rtype_error))
+evaluate_dec_i1 genv cenv (s1,tdecs) (Dlet_i1 n e) ((s2,tdecs), Rerr Rtype_error))
 
-/\ (! genv cenv n e err s count s'.
+/\ (! genv cenv n e err s count s' tdecs.
 (evaluate_i1 F (genv,cenv,emp) ( 0,s) e ((count,s'), Rerr err))
 ==>
-evaluate_dec_i1 genv cenv s (Dlet_i1 n e) (s', Rerr err))
+evaluate_dec_i1 genv cenv (s,tdecs) (Dlet_i1 n e) ((s',tdecs), Rerr err))
 
 /\ (! genv cenv funs s.
 T
 ==>
 evaluate_dec_i1 genv cenv s (Dletrec_i1 funs) (s, Rval (emp, MAP (\ (f,x,e) .  Closure_i1 (cenv,[]) x e) funs)))
 
-/\ (! mn genv cenv tds s.
-(check_dup_ctors tds)
+/\ (! mn genv cenv tds s tdecs new_tdecs.
+(check_dup_ctors tds /\
+((new_tdecs = type_defs_to_new_tdecs mn tds) /\
+DISJOINT new_tdecs tdecs))
 ==>
-evaluate_dec_i1 genv cenv s (Dtype_i1 mn tds) (s, Rval (build_tdefs mn tds, [])))
+evaluate_dec_i1 genv cenv (s,tdecs) (Dtype_i1 mn tds) ((s,(new_tdecs UNION tdecs)), Rval (build_tdefs mn tds, [])))
 
-/\ (! mn genv cenv tds s.
-(~ (check_dup_ctors tds))
+/\ (! mn genv cenv tds s tdecs.
+(~ (check_dup_ctors tds) \/
+~ (DISJOINT (type_defs_to_new_tdecs mn tds) tdecs))
 ==>
-evaluate_dec_i1 genv cenv s (Dtype_i1 mn tds) (s, Rerr Rtype_error))
+evaluate_dec_i1 genv cenv (s,tdecs) (Dtype_i1 mn tds) ((s,tdecs), Rerr Rtype_error))
 
-/\ (! mn genv cenv cn ts s.
-T
+/\ (! mn genv cenv cn ts s tdecs.
+(~ (TypeExn (mk_id mn cn) IN tdecs))
 ==>
-evaluate_dec_i1 genv cenv s (Dexn_i1 mn cn ts) (s, Rval (bind cn (LENGTH ts, TypeExn (mk_id mn cn)) emp, [])))`;
+evaluate_dec_i1 genv cenv (s,tdecs) (Dexn_i1 mn cn ts) ((s, ({TypeExn (mk_id mn cn)} UNION tdecs)), Rval (bind cn (LENGTH ts, TypeExn (mk_id mn cn)) emp, [])))
+
+/\ (! mn genv cenv cn ts s tdecs.
+(TypeExn (mk_id mn cn) IN tdecs)
+==>
+evaluate_dec_i1 genv cenv (s,tdecs) (Dexn_i1 mn cn ts) ((s,tdecs), Rerr Rtype_error))`;
 
 val _ = Hol_reln ` (! genv cenv s.
 T
@@ -734,28 +742,21 @@ evaluate_decs_i1 (genv ++ new_env) (merge_envC (emp,new_tds) cenv) s2 ds (s3, ne
 ==>
 evaluate_decs_i1 genv cenv s1 (d::ds) (s3, merge new_tds' new_tds, (new_env ++ new_env'), r))`;
 
- val _ = Define `
-
-(dec_to_cenv_i1 (Dtype_i1 mn tds) = (build_tdefs mn tds))
-/\
-(dec_to_cenv_i1 (Dexn_i1 mn cn ts) = (bind cn (LENGTH ts,TypeExn (mk_id mn cn)) emp))
-/\
-(dec_to_cenv_i1 _ = ([]))`;
-
-
- val _ = Define `
-
-(decs_to_cenv_i1 [] = ([]))
-/\
-(decs_to_cenv_i1 (d::ds) = (decs_to_cenv_i1 ds ++ dec_to_cenv_i1 d))`;
-
-
 (*val mod_cenv : maybe modN -> flat_envC -> envC*)
 val _ = Define `
  (mod_cenv mn cenv =  
 ((case mn of
       NONE => ([],cenv)
     | SOME mn => ([(mn,cenv)],[])
+  )))`;
+
+
+(*val update_mod_state : maybe modN -> set modN -> set modN*)
+val _ = Define `
+ (update_mod_state mn mods =  
+((case mn of
+      NONE => mods
+    | SOME mn => {mn} UNION mods
   )))`;
 
 
@@ -775,15 +776,16 @@ val _ = Define `
 (decs_to_dummy_env (d::ds) = (decs_to_dummy_env ds + dec_to_dummy_env d))`;
 
 
-val _ = Hol_reln ` (! genv cenv s1 ds s2 cenv' env mn.
-(evaluate_decs_i1 genv cenv s1 ds (s2,cenv',env,NONE))
+val _ = Hol_reln ` (! genv cenv s1 tdecs1 mods ds s2 tdecs2 cenv' env mn.
+(evaluate_decs_i1 genv cenv (s1,tdecs1) ds ((s2,tdecs2),cenv',env,NONE))
 ==>
-evaluate_prompt_i1 genv cenv s1 (Prompt_i1 mn ds) (s2, mod_cenv mn cenv', env, NONE))
+evaluate_prompt_i1 genv cenv (s1,tdecs1,mods) (Prompt_i1 mn ds) ((s2,tdecs2,update_mod_state mn mods), mod_cenv mn cenv', env, NONE))
 
-/\ (! genv cenv s1 mn ds s2 cenv' env err.
-(evaluate_decs_i1 genv cenv s1 ds (s2,cenv',env,SOME err))
+/\ (! genv cenv s1 tdecs1 mods mn ds s2 tdecs2 cenv' env err.
+(evaluate_decs_i1 genv cenv (s1,tdecs1) ds ((s2,tdecs2),cenv',env,SOME err))
 ==>
-evaluate_prompt_i1 genv cenv s1 (Prompt_i1 mn ds) (s2, 
+evaluate_prompt_i1 genv cenv (s1,tdecs1,mods) (Prompt_i1 mn ds) 
+                                                  ((s2,tdecs2,update_mod_state mn mods),
                                                    mod_cenv mn cenv',                                                   
  (env ++ GENLIST (\n .  
   (case (n ) of ( _ ) => Litv_i1 Unit )) (decs_to_dummy_env ds - LENGTH env)),
